src/Language/PlutusIR/DecOpt.v
@@ -7,14 +7,3 @@ From QuickChick Require Import QuickChick.
 
 QCDerive EnumSized for DefaultUni.
 QCDerive EnumSized for Strictness.
-
-(* FIXME: Mock instance, here temporary. If not removed, might cause QuickChick to derive computation
-    that does not actually function properly *)
-Instance EnumSizedstring : EnumSized string :=
-  {| enumSized _ := ret EmptyString |}.
-
-Instance EnumSizedTy : EnumSized Ty :=
-  {| enumSized _ := ret (Ty_Var EmptyString) |}.
-
-Instance EnumSizedTerm : EnumSized Term :=
-  {| enumSized _ := ret (Var EmptyString) |}.
